---
title: "Perturbing the Euler-Lagrange equations for calculus of variations: a first-order analysis"
author: "Robin Hankin"
output: pdf_document
---


```{r setup, include=FALSE}
knitr::opts_chunk$set(echo = TRUE)
```

\newcommand{\di}[2]{\frac{\partial{#1}}{\partial{#2}}}

Consider a perturbation:

\begin{eqnarray}
y  &\longrightarrow&  y(x) + \epsilon z(x)\\
y' &\longrightarrow&  y'(x) + \epsilon z'(x)\\
F  &\longrightarrow&  F + \epsilon G(x,y,y')
\end{eqnarray}


\begin{equation} 
\frac{d}{dx}\di{F}{y'}=\di{F}{y}\longrightarrow
\frac{d}{dx}\left[\di{}{y'}\left(F(x,y+\epsilon z,y'+\epsilon z')+\epsilon G(x,y+\epsilon z,y'+\epsilon z')\right)\right] =
\di{}{y}\left[F+\epsilon G(x,y+\epsilon z,y'+\epsilon z')\right]
\end{equation}

Above we write $y$ for $y(x)$ etc.  We have to remember that
$y,y',z,z'$ are functions of $x$.  Now neglect terms of order
$\epsilon^2$ and above, and continue to neglect them:

\begin{equation}
\frac{d}{dx}\left[\di{}{y'}\left(F(x,y+\epsilon z,y'+\epsilon z')+\epsilon G(x,y,y')\right)\right] =
\di{}{y}\left[F+\epsilon G(x,y,y')\right]
\end{equation}

\begin{equation}
\frac{d}{dx}\left[\di{}{y'}\left(
F(x,y,y') + \epsilon z\di{F}{y}+ \epsilon z'\di{F}{y'}
+\epsilon G(x,y,y')\right)\right] =
\di{}{y}\left[F+\epsilon G(x,y,y')\right]
\end{equation}

The $\epsilon^0$ term is just the Euler-Lagrange equation, which is
known to be true.  The first order term is:

\begin{equation}\label{EL1}
\frac{d}{dx}\left[\di{}{y'}\left(
z\di{F}{y} + z'\di{F}{y'} + G\right)\right] =
\di{G}{y}
\end{equation}

(above we have to remember that $G=G(x,y,y')$). 
As a consistency check, we set $G=F$:

\begin{equation}\label{ELeq}
\frac{d}{dx}\left[\di{}{y'}\left(
z\di{F}{y} + z'\di{F}{y'} + F\right)\right] =
\di{F}{y}
\end{equation}

As an example, we will take $F=\sqrt{1+y'^2}$:


\begin{equation}
\frac{d}{dx}\left[\di{}{y'}\left(
\frac{z'y'}{\sqrt{1+y'^2}} + \sqrt{1+y'^2}\right)\right] =
0
\end{equation}

\begin{equation}
\frac{d}{dx}\left[
\frac{z'}{\sqrt{1+y'^2}^{3/2}} + \frac{y'}{1+y'^2}\right] =
0
\end{equation}

Now note that $y'$ is a constant, say $s$ for slope, giving 

\begin{equation}
z''=0\longrightarrow z=c_1 + c_2x
\end{equation}

and the boundary conditions give $c_1=c_2=0$.



\section{Beltrami identity}


This is

\begin{equation}\label{beltrami}
F-u'\di{F}{y'}=C
\end{equation}

and we apply the same perturbation as before, specifically
$F\longrightarrow F+\epsilon G$.  Taking the first order terms and
subtracting out Beltrami we get

\begin{equation}\label{beltrami_epsilon}
G-y'\di{G}{y'}-z'\di{F}{y'}=C
\end{equation}

for some (other) constant $C$.  Apply $F=\sqrt{1+y'^2}$ to
equation \ref{beltrami} gives

\begin{equation}
\sqrt{1+y'^2}-\frac{y'^2}{\sqrt{1+y'^2}}=C
\end{equation}

Simplifying:

\begin{equation}
\sqrt{1+y'^2}=1/C
\end{equation}

or 

\begin{equation}\label{straightline}
y'= K
\end{equation}

for $K$ some constant.  Now perturb it with $G=f(y)$ and substitute
into equation \ref{beltrami_epsilon}:

\begin{equation}
f(y) - \frac{z'y'}{\sqrt{1+y'^2}}=C
\end{equation}

\begin{equation}
f(y) - sz'=C
\end{equation}

(where $s=K/\sqrt{1+K^2}$, a constant).  Integrating

\begin{equation}
z' = \frac{f(y)-C}{s}
\end{equation}

But we know that y=y_0 + \frac{x-x_0}{y_1-y_0}



